@prefix odrl:   <http://www.w3.org/ns/odrl/2/> .
@prefix rdfs:   <http://www.w3.org/2000/01/rdf-schema#> .
@prefix report: <https://w3id.org/force/compliance-report#> .
@prefix skos:   <http://www.w3.org/2004/02/skos/core#> .
@prefix sotw:   <https://ex.org/sotw#> .
@prefix xsd:    <http://www.w3.org/2001/XMLSchema#> .

sotw:SotW a rdfs:Class, skos:Concept ;
    rdfs:isDefinedBy sotw: ;
    rdfs:label "State of the World"@en ;
    skos:definition "A set of knowledge representing real-world information aiding the evaluation of ODRL Policies"@en .

sotw:currentTime a rdfs:Property, skos:Concept ;
    rdfs:isDefinedBy sotw: ;
    skos:definition "Denotes the current time of the state of the world"@en ;
    rdfs:domain sotw:SotW ;
    rdfs:range xsd:date, xsd:dateTime .

sotw:location a rdfs:Property, skos:Concept ;
    rdfs:isDefinedBy sotw: ;
    skos:definition "Denotes the location where the policy is being evaluated"@en ;
    rdfs:domain sotw:SotW .

sotw:assetCollection a rdfs:Property, skos:Concept ;
    rdfs:isDefinedBy sotw: ;
    skos:definition "Denotes an asset that is part of an asset collection"@en ;
    rdfs:domain sotw:SotW ;
    rdfs:range odrl:Asset .

sotw:partyCollection a rdfs:Property, skos:Concept ;
    rdfs:isDefinedBy sotw: ;
    skos:definition "Denotes a party that is part of a party collection"@en ;
    rdfs:domain sotw:SotW ;
    rdfs:range odrl:Party .

sotw:report a rdfs:Property, skos:Concept ;
    rdfs:isDefinedBy sotw: ;
    skos:definition "Denotes existing reports from previously performed ODRL evaluations"@en ;
    skos:note "Previous reports can be used to get history of attempted and performed actions"@en ;
    rdfs:domain sotw:SotW ;
    rdfs:range report:PolicyReport .

sotw:count a rdfs:Property, skos:Concept ;
    rdfs:isDefinedBy sotw: ;
    skos:definition "Denotes the amount of times a rule has been exercised"@en ;
    rdfs:domain sotw:SotW .

sotw:event a rdfs:Property, skos:Concept ;
    rdfs:isDefinedBy sotw: ;
    skos:definition "Denotes information about an event that has occurred, e.g., when it has occurred"@en ;
    rdfs:domain sotw:SotW .

sotw:accumulatedTime a rdfs:Property, skos:Concept ;
    rdfs:isDefinedBy sotw: ;
    skos:definition "Denotes an accumulated amount of time a rule has been exercised"@en ;
    rdfs:domain sotw:SotW ;
    rdfs:range xsd:duration .

sotw:recipient a rdfs:Property, skos:Concept ;
    rdfs:isDefinedBy sotw: ;
    skos:definition "Denotes information about a recipient of a rule that has been exercised"@en ;
    rdfs:domain sotw:SotW .
